up to ps5

pset01_ProgramAnalysis/Pset1Implementation.v
@@ -19,8 +19,11 @@ Module Impl.
   (* Define [Neg] so that it implements Boolean negation, which flips
    * the truth value of a Boolean value.
    *)
-  Definition Neg (b : bool) : bool.
-  Admitted.
+  Definition Neg (b : bool) : bool:=
+    match b with
+    | true => false
+    | false => true
+    end.
 
   (* For instance, the negation of [true] should be [false].
    * This proof should follow from reducing both sides of the equation
@@ -28,7 +31,9 @@ Module Impl.
    *)
   Theorem Neg_true : Neg true = false.
   Proof.
-  Admitted.
+    simplify.
+    linear_arithmetic.
+  Qed.
 
   (* Negation should be involutive, meaning that if we negate
    * any Boolean value twice, we should get the original value back.
@@ -39,43 +44,64 @@ Module Impl.
    *)
   Theorem Neg_involutive : forall b : bool, Neg (Neg b) = b.
   Proof.
-  Admitted.
+    simplify.
+    cases (b).
+
+    equality.
+    equality.
+  Qed.
 
   (* Define [And] so that it implements Boolean conjunction. That is,
    * the result value should be [true] exactly when both inputs
    * are [true].
    *)
-  Definition And (x y : bool) : bool.
-  Admitted.
+  Definition And (x y : bool) : bool :=
+    match x, y with
+      | true, true => true
+      | _, _ => false
+    end.
 
   (* Here are a couple of examples of how [And] should act on
    * concrete inputs.
    *)
   Theorem And_true_true : And true true = true.
   Proof.
-  Admitted.
+    simplify.
+    linear_arithmetic.
+  Qed.
 
   Theorem And_false_true : And false true = false.
   Proof.
-  Admitted.
+    simplify.
+    linear_arithmetic.
+  Qed.
 
   (* Prove that [And] is commutative, meaning that switching the order
    * of its arguments doesn't affect the result.
    *)
   Theorem And_comm : forall x y : bool, And x y = And y x.
   Proof.
-  Admitted.
+    simplify.
+    cases(x).
+    equality; simplify.
+
+    cases(y).
+    equality. equality.
+  Qed.
 
   (* Prove that the conjunction of a Boolean value with [true]
    * doesn't change that value.
    *)
   Theorem And_true_r : forall x : bool, And x true = x.
   Proof.
-  Admitted.
+    simplify.
+    cases(x).
+    equality. simplify. equality.
+  Qed.
 
   (* You may have noticed that the [=] operator above does not return a [bool]. *)
   Check (true = false).
-  
+
   (* [a = b] is instead a [Prop], short for proposition, the type of logical
    * statements. The set of propositions in Rocq is large and contains a variety
    * of statements, many of which are undecideable, so we can't in general
@@ -87,7 +113,7 @@ Module Impl.
    *)
   Compute (if 1 ==n 2 then (And true false) else true).
   Compute (1 = 2 -> True /\ False).
-  
+
   (* The following operations that you have seen or will see soon are in [Prop],
    * so they cannot be used in if-then-else statements:
    * - [a = b] (equality at an arbitrary type)
@@ -108,24 +134,25 @@ Module Impl.
    * To see an example of what can go wrong, uncommment the following [Compute] command
    * and note the reported error message.
    *)
-  
-  (* Compute if 0 < 1 then 0 else 1. *)
+
+  (*Compute if 0 < 1 then 0 else 1.*)
+  (*!!! The term "0 < 1" has type "Prop" which is not a (co-)inductive type.*)
 
   (* The correct boolean version. *)
   Compute if Nat.ltb 0 1 then 0 else 1.
-  
+
   (* In the second part of this assignment, we will work with a simple language
    * of imperative arithmetic programs that sequentially apply operations
    * to a natural-number-valued state.
-   * 
+   *
    * Remember that we are working with natural division which rounds down.
    * Note the output of these [Compute] commands.
    *)
-  
+
   Compute 3 / 3.
   Compute 2 / 3.
   Compute 4 / 3.
-  
+
   (*
 
    * The [Prog] datatype defines abstract syntax trees for this language.
@@ -137,43 +164,74 @@ Module Impl.
    * that running the program [p] should result in, when the
    * initial state is [n].
    *)
-  Fixpoint run (p : Prog) (initState : nat) : nat.
-  Admitted.
+  Fixpoint run (p : Prog) (initState : nat) : nat :=
+    match p with
+      | Done => initState
+      | AddThen n subp => run subp (initState + n)
+      | MulThen n subp => run subp (n * initState)
+      | DivThen n subp => run subp (initState / n)
+      | VidThen n subp => run subp (n / initState)
+      | SetToThen n subp => run subp n
+    end.
 
   Theorem run_Example1 : run Done 0 = 0.
   Proof.
-  Admitted.
+    simplify.
+    linear_arithmetic.
+  Qed.
 
   Theorem run_Example2 : run (MulThen 5 (AddThen 2 Done)) 1 = 7.
   Proof.
-  Admitted.
+    simplify.
+    linear_arithmetic.
+  Qed.
 
   Theorem run_Example3 : run (SetToThen 3 (MulThen 2 Done)) 10 = 6.
   Proof.
-  Admitted.
+    simplify.
+    linear_arithmetic.
+  Qed.
 
   (* Define [numInstructions] to compute the number of instructions
    * in a program, not counting [Done] as an instruction.
    *)
-  Fixpoint numInstructions (p : Prog) : nat.
-  Admitted.
+  Fixpoint numInstructions (p : Prog) : nat :=
+    match p with
+      | Done => 0
+      | AddThen _ p => 1 + numInstructions p
+      | MulThen _ p => 1 + numInstructions p
+      | DivThen _ p => 1 + numInstructions p
+      | VidThen _ p => 1 + numInstructions p
+      | SetToThen _ p => 1 + numInstructions p
+    end.
 
   Theorem numInstructions_Example :
     numInstructions (MulThen 5 (AddThen 2 Done)) = 2.
   Proof.
-  Admitted.
+    simplify.
+    linear_arithmetic.
+  Qed.
 
   (* Define [concatProg] such that [concatProg p1 p2] is the program
    * that first runs [p1] and then runs [p2].
    *)
-  Fixpoint concatProg (p1 p2 : Prog) : Prog.
-  Admitted.
+  Fixpoint concatProg (p1 p2 : Prog) : Prog :=
+    match p1 with
+      | Done => p2
+      | AddThen n p => AddThen n (concatProg p p2)
+      | MulThen n p => MulThen n (concatProg p p2)
+      | DivThen n p => DivThen n (concatProg p p2)
+      | VidThen n p => VidThen n (concatProg p p2)
+      | SetToThen n p => SetToThen n (concatProg p p2)
+    end.
 
   Theorem concatProg_Example :
        concatProg (AddThen 1 Done) (MulThen 2 Done)
        = AddThen 1 (MulThen 2 Done).
   Proof.
-  Admitted.
+    simplify.
+    equality.
+  Qed.
 
   (* Prove that the number of instructions in the concatenation of
    * two programs is the sum of the number of instructions in each
@@ -183,7 +241,8 @@ Module Impl.
     : forall (p1 p2 : Prog), numInstructions (concatProg p1 p2)
                         = numInstructions p1 + numInstructions p2.
   Proof.
-  Admitted.
+    induct p1; simplify; try rewrite IHp1; linear_arithmetic.
+  Qed.
 
   (* Prove that running the concatenation of [p1] with [p2] is
      equivalent to running [p1] and then running [p2] on the
@@ -193,7 +252,8 @@ Module Impl.
       run (concatProg p1 p2) initState =
       run p2 (run p1 initState).
   Proof.
-  Admitted.
+    induct p1; simplify; try rewrite IHp1; linear_arithmetic.
+Qed.
 
   (* Read this definition and understand how division by zero is handled. *)
   Fixpoint runPortable (p : Prog) (state : nat) : bool * nat :=
@@ -235,7 +295,22 @@ Module Impl.
   Lemma runPortable_run : forall p s0 s1,
     runPortable p s0 = (true, s1) -> run p s0 = s1.
   Proof.
-  Admitted.
+    induct p.
+    simplify. equality.
+
+    simplify. apply IHp in H. try rewrite Nat.add_comm. equality.
+    simplify. apply IHp in H. equality.
+
+    simplify.
+    cases (n ==n 0).
+    equality. apply IHp in H. equality.
+
+    simplify.
+    cases (s0 ==n 0).
+    equality. apply IHp in H. equality.
+
+    simplify. apply IHp in H. equality.
+  Qed.
 
   (* The final goal of this pset is to implement [validate : Prog -> bool]
      such that if this function returns [true], the program would not trigger
@@ -270,28 +345,62 @@ Module Impl.
    * succeed. Some may call Rocq a video game, but it is not a grinding contest. *)
 
 
-  Definition validate (p : Prog) : bool.
-  Admitted.
+  (* Definition validate (p : Prog) : bool.
+  Admitted. *)
+  Compute 2-10.
+  (* HINT 1: *)
+  (*   Definition validate p := validate' p false. *)
+  (*   Fixpoint validate' (p : Prog) (nz : bool) : bool. Admitted. *)
+          (* if [nz=true], [validate'] can assume that the [state] on which
+            [p] will be run is nonzero. When calling [validate']
+            recursively, take care to pass in [nz] that corresponds to the
+            state after the current operation. *)
+
+  Fixpoint validate' (p : Prog) (nz : bool) : bool :=
+    match p with
+      | Done => true
+      | AddThen n subp => validate' subp (if n ==n 0 then nz else true)
+      | MulThen n subp => validate' subp (if n ==n 0 then false else nz)
+      | DivThen n subp => if n ==n 0 then false else if n ==n 1 then validate' subp nz else validate' subp false
+      | VidThen n subp => if nz then validate' subp false else false
+      | SetToThen n subp => validate' subp (if n ==n 0 then false else true)
+    end.
+
+  Definition validate (p : Prog) : bool := validate' p false.
+
 
   (* Start by making sure that your solution passes the following tests, and add
    * at least one of your own tests: *)
 
-  Example validate1 : validate goodProgram1 = true. Admitted.
-  Example validate2 : validate goodProgram2 = true. Admitted.
-  Example validate3 : validate goodProgram3 = true. Admitted.
-  Example validate4 : validate goodProgram4 = true. Admitted.
-  Example validate5 : validate goodProgram5 = true. Admitted.
-  Example validate6 : validate goodProgram6 = true. Admitted.
-  Example validate7 : validate goodProgram7 = true. Admitted.
-  Example validateb1 : validate badProgram1 = false. Admitted.
-  Example validateb2 : validate badProgram2 = false. Admitted.
+  Example validate1 : validate goodProgram1 = true.
+  Proof. equality. Qed.
+  Example validate2 : validate goodProgram2 = true.
+  Proof. equality. Qed.
+  Example validate3 : validate goodProgram3 = true.
+  Proof. equality. Qed.
+  Example validate4 : validate goodProgram4 = true.
+  Proof. equality. Qed.
+  Example validate5 : validate goodProgram5 = true.
+  Proof. equality. Qed.
+  Example validate6 : validate goodProgram6 = true.
+  Proof. equality. Qed.
+  Example validate7 : validate goodProgram7 = true.
+  Proof. equality. Qed.
+  Definition goodProgram8 : Prog := (SetToThen 0 (AddThen 2 (DivThen 3 Done))).
+  Example validate8 : validate goodProgram8 = true.
+  Proof. equality. Qed.
+
+  Example validateb1 : validate badProgram1 = false.
+  Proof. equality. Qed.
+  Example validateb2 : validate badProgram2 = false.
+  Proof. equality. Qed.
 
   (* Then, add your own example of a bad program here, and check that `validate`
    * returns `false` on it: *)
 
-  Definition badProgram3 : Prog. Admitted.
-  Example validateb3 : validate badProgram3 = false. Admitted.
-
+  Definition badProgram3 := AddThen 2 (DivThen 3 (VidThen 2 Done)).
+  Example validateb3 : validate badProgram3 = false.
+  Proof. equality. Qed.
 
 
   (* Finally, before diving into the Rocq proof, try to convince yourself that
@@ -302,13 +411,93 @@ Module Impl.
    * proceeding. *)
 
   (** Proof sketch: **)
-  (* [[Fill in your proof sketch here.]] *)
+  (* [[
+  Definition P (p : Prog) :=
+       (validate' p true = true ->
+        forall s, s <> 0 -> runPortable p s = (true, run p s)) /\
+       (validate' p false = true ->
+        forall s, runPortable p s = (true, run p s)).
+    denote the flag as nz
+    IH = P.
+    Base case:
+      Done - trivial
+    Inductive step:
+      cases:
+        AddThen n subp:
+            n == 0: [validate' (AddThen n subp) nz] = [validate' subp nz]. By IH and runPortable_run lemma, voila.
+            (when n is zero, only care about state nz)
+            n != 0: [validate' (AddThen n subp) nz] = [validate' subp true]. By IH and runPortable_run lemma, voila.
+            (when n is non-zero, state doesn't matter as sum is guaranteed to be positive).
+        MulThen n subp:
+            n == 0: [validate' (MulThen n subp) nz] = [validate' subp false]. By IH and runPortable_run lemma, voila.
+            (when n is zero, our new state is gonna be zero, so no matter nz was, for subproblem, new nz is false)
+            n != 0: [validate' (MulThen n subp) nz] = [validate' subp nz]. By IH and runPortable_run lemma, voila.
+            (when n is non-zero, we care about previous state - so for subproblem we pass old nz).
+        DivThen n subp:
+            n == 0: div by zero abort - not very interesting one.
+            n == 1: [validate' (DivThen n subp) nz] = [validate' subp nz] By IH and runPortable_run lemma, voila
+            (dividing by 1 doesnt change state, so IH applies with same nz).
+            n > 1: [validate' (DivThen n subp) nz] = [validate' subp false]. By IH and runPortable_run lemma, voila
+            (now even thoug its positive the division could yield zero like 2/3).
+          VidThen n subp (divide n by state):
+            if state is nonzero (nz=true), [validate' (VidThen n subp)] = validate' subp false - new nz is false as we
+            still might end up with division yielding zero (if n is zero or n < state like 2/3)
+            state is zero (nz==false), then abort with false.
+        SetToThen n subp: state becomes n.
+            n == 0: [validate' (SetToThen n subp) nz] = [validate' subp false] By IH and runPortable_run lemma, voila
+            (setting to zero means directly next nz is false)
+            n != 0: [validate' (SetToThen n subp) nz] = [validate' subp true] By IH and runPortable_run lemma, voila
+            (setting to nonzero means directly next nz is true)
+  ]] *)
 
   (* Now you're ready to write the proof in Rocq: *)
+  Definition P (p : Prog) :=
+       (validate' p true = true ->
+        forall s, s <> 0 -> runPortable p s = (true, run p s)) /\
+       (validate' p false = true ->
+        forall s, runPortable p s = (true, run p s)).
+
+  Lemma P_holds : forall p, P p.
+  Proof.
+    unfold P.
+    induct p; simplify.
+    - propositional.
+    - simplify.
+      cases (n ==n 0).
+        rewrite e. simplify. propositional. rewrite Nat.add_0_r. apply H2. linear_arithmetic. rewrite Nat.add_0_r. apply H2.
+        propositional. simplify. rewrite Nat.add_comm. apply H2. linear_arithmetic. rewrite Nat.add_comm. apply H2. linear_arithmetic.
+
+    - simplify.
+      cases (n ==n 0).
+        rewrite e. simplify. propositional. apply H2. apply H2.
+        simplify. propositional. apply H2. linear_arithmetic. apply H2.
+
+    - cases (n ==n 0).
+        rewrite e. propositional. linear_arithmetic.
+        linear_arithmetic.
+
+      cases (n ==n 1).
+        rewrite e. propositional. rewrite Nat.div_1_r. apply H2. linear_arithmetic. rewrite Nat.div_1_r. apply H2.
+
+      propositional. apply H2. cases (s ==n 0). rewrite e. Search (0/_). rewrite Nat.Div0.div_0_l. apply H2. apply H2.
+
+    - simplify. propositional.
+      cases (s ==n 0).
+        linear_arithmetic.
+        apply H2. linear_arithmetic.
+
+    - simplify.
+      cases (n ==n 0).
+        propositional. apply H2. apply H2.
+        propositional. apply H2. linear_arithmetic. apply H2. linear_arithmetic.
+  Qed.
 
   Lemma validate_sound : forall p, validate p = true ->
     forall s, runPortable p s = (true, run p s).
-  Admitted.
+  Proof.
+    apply P_holds.
+
+  Qed.
 
   (* Here is the complete list of commands used in one possible solution:
     - Search, for example Search (_ + 0).
