pset02_BinomialCoefficients/Pset2.v
@@ -57,13 +57,13 @@ Module Impl.
      because the recursive call [fact_nat n'] operates on [n'], which is a subterm
      of [n].
    *)
-  
+
   Fixpoint fact_nat (n : nat) : nat :=
     match n with
     | O => 1
     | S n' => (n' + 1) * (fact_nat n')
     end.
-  
+
   (*
      In this pset, however, we want to use the binary representation of natural
      numbers, which is called "N" in Rocq.  This representation stores numbers as
@@ -135,14 +135,25 @@ Module Impl.
   (* Exercise: Define a simple exponentiation function in the same style, so that
      "exp base n" equals "base^n". *)
 
-  Definition exp(base: N): N -> N. Admitted.
+  Definition exp(base: N): N -> N :=
+    recurse by cases
+    | 0 => 1
+    | n + 1 => base * recurse
+    end.
 
   (* Once you define "exp", you can replace "Admitted." below by "Proof. equality. Qed." *)
-  Lemma test_exp_2_3: exp 2 3 = 8. Admitted.
-  Lemma test_exp_3_2: exp 3 2 = 9. Admitted.
-  Lemma test_exp_4_1: exp 4 1 = 4. Admitted.
-  Lemma test_exp_5_0: exp 5 0 = 1. Admitted.
-  Lemma test_exp_1_3: exp 1 3 = 1. Admitted.
+  Lemma test_exp_2_3: exp 2 3 = 8.
+  Proof. equality. Qed.
+  Lemma test_exp_3_2: exp 3 2 = 9.
+  Proof. equality. Qed.
+  Lemma test_exp_4_1: exp 4 1 = 4.
+  Proof. equality. Qed.
+  Lemma test_exp_5_0: exp 5 0 = 1.
+  Proof. equality. Qed.
+  Lemma test_exp_1_3: exp 1 3 = 1.
+  Proof. equality. Qed.
+  Lemma test_exp_2_8: exp 2 8 = 256.
+  Proof. equality. Qed.
 
   (* Here's another recursive function defined in the same style to apply a
      function f to a range of values:
@@ -154,6 +165,7 @@ Module Impl.
     end.
 
   Compute (seq (fun x => x * x) 4 10).
+  (*seq f  a b = [f(a), f(a+1), ..., f(a+b-1)]*)
 
   (* "ith i l" returns the i-th element of the list l.
      To understand the recursion, note that "ith i" returns a function that takes
@@ -222,6 +234,7 @@ Module Impl.
       simplify. rewrite IHcount. linear_arithmetic.
   Qed.
 
+
   (* And here's another general hint: You don't always need induction.  Some lemmas
      in this pset can be solved using induction but don't actually require it
      and are simpler to solve if you don't use induction, so before doing
@@ -231,12 +244,43 @@ Module Impl.
   Lemma seq_spec: forall f count i start, i < count -> ith i (seq f count start) = f (start + i).
   Proof.
     induct count; simplify.
-  Admitted.
+    linear_arithmetic.
+
+    unfold_recurse (seq f) count.
+
+    cases i.
+
+    simplify.
+    Search(_+0).
+    rewrite N.add_0_r.
+    linear_arithmetic.
+
+    unfold_recurse ith i.
+
+    assert (i < count) by linear_arithmetic.
+    rewrite IHcount by assumption.
+    replace (start + 1 + i) with (start + (i + 1)) by linear_arithmetic.
+    reflexivity.
+  Qed.
+
 
   (* Exercise: Prove that if the index is out of bounds, "ith" returns 0. *)
   Lemma ith_out_of_bounds_0: forall i l, len l <= i -> ith i l = 0.
   Proof.
-  Admitted.
+    induct i; simplify.
+
+    cases l; simplify; linear_arithmetic.
+
+    cases l.
+
+    simplify; unfold_recurse ith i; linear_arithmetic.
+
+    unfold_recurse ith i.
+    simplify.
+    apply IHi.
+    linear_arithmetic.
+
+  Qed.
 
 
   (* Binomial coefficients *)
@@ -307,7 +351,7 @@ Module Impl.
      tactic "nia" (which stands for "non-linear integer arithmetic"), but it does
      not always work, so sometimes you will have to search for appropriate lemmas
      to apply manually.  For instance, to prove the following: *)
-  Goal forall n m, n <> 0 -> m <> 0 -> n * m <> 0.
+  Lemma mul_nonneg: forall n m, n <> 0 -> m <> 0 -> n * m <> 0.
   Proof.
     simplify.
     (* you could use the "Search" command with a pattern: *)
@@ -321,7 +365,7 @@ Module Impl.
 
   (* Here's another example of how to use the "Search" command: Suppose you have
      the goal *)
-  Goal forall n, n <> 0 -> n / n = 1.
+  Lemma div_1: forall n, n <> 0 -> n / n = 1.
   Proof.
     simplify.
     (* If we do "Search (_ / _)" we get a very long list, but if we do *)
@@ -335,15 +379,40 @@ Module Impl.
 
   Lemma fact_nonzero: forall n, n! <> 0.
   Proof.
-  Admitted.
+    simplify.
+    induct n.
+    simplify.
+    linear_arithmetic.
+
+    unfold_recurse fact n.
+    Search (_ * _ <> 0).
+    apply N.neq_mul_0.
+    linear_arithmetic.
+  Qed.
 
   Lemma Cn0: forall n, C n 0 = 1.
   Proof.
-  Admitted.
+    simplify.
+    induct n. equality.
+    unfold C.
+    simplify. Search(_*1). rewrite N.mul_1_r.
+    Search(_-0). rewrite N.sub_0_r.
+    apply div_1.
+    apply fact_nonzero.
+  Qed.
 
   Lemma Cnn: forall n, C n n = 1.
   Proof.
-  Admitted.
+    simplify.
+    unfold C.
+    simplify.
+    Search(_-_).
+    rewrite N.sub_diag.
+    simplify.
+    rewrite N.mul_1_l.
+    apply N.div_same.
+    apply fact_nonzero.
+  Qed.
 
 
   (* It's somewhat surprising that in the definition of C(n, k),
@@ -479,10 +548,69 @@ Module Impl.
      "a / b * c / d" is "((a / b) * c) / d", NOT "(a / b) * (c / d)"
 
   Here we go: *)
+  Compute C 0 1.
+
+  Lemma unfold_fact: forall n k, k + 1 <= n-> (n - k)! = (n - k - 1)! * (n - k).
+  Proof.
+    simplify.
+    assert (H1: n - k <> 0).
+    linear_arithmetic.
+    replace (n - k) with (n - k - 1 + 1) by linear_arithmetic.
+    unfold_recurse fact (n-k-1).
+    rewrite N.mul_comm.
+    replace (n - k - 1 + 1 - 1) with (n - k - 1) by linear_arithmetic.
+    equality.
+  Qed.
+
+  Compute 0 - 1 + 1.
+
+  (* Lemma Cn1: forall n, C n 1 = n. *)
+  Lemma Cnk_1: forall n k, k + 1 <= n-> C n (k+1) = C n k * (n - k) / (k + 1).
+  Proof.
+    simplify.
+    unfold C.
+
+    replace (n - (k + 1)) with (n - k - 1) by linear_arithmetic.
+
+    unfold_recurse fact k.
+    rewrite N.mul_assoc.
+
+    replace ((n - k)!) with ((n - k - 1 + 1)!) by (f_equal; linear_arithmetic).
+
+    unfold_recurse fact (n-k-1).
+
+    replace (n - k - 1 + 1) with (n - k) by linear_arithmetic.
+
+    assert ((n - k - 1)! * (n - k) * k! | n!).
+    replace ((n - k - 1)! * (n - k)) with ((n-k)!) by (rewrite unfold_fact; linear_arithmetic).
+    apply C_is_integer; linear_arithmetic.
+
+    Search(_/_*_).
+    symmetry.
+    replace (n! / ((n - k) * (n - k-1)! * k!) * (n - k))  with (n! * (n-k) / ((n - k - 1)! * (n - k) * k!)).
+    replace ((n - k - 1)! * (n - k) * k!) with (((n - k - 1)! * k!)*(n - k)) by nia.
+    Search(_*_/(_*_)).
+    rewrite N.Div0.div_mul_cancel_r by linear_arithmetic.
+    Search(_/_/_).
+    rewrite N.Div0.div_div.
+
+    Search(_*_*_). rewrite N.mul_shuffle0. equality.
+    replace (n! * (n - k)) with ((n - k)*n!) by nia.
+    rewrite N.Lcm0.divide_div_mul_exact by (apply H0).
+    rewrite N.mul_comm.
+    replace ((n - k - 1)! * (n - k)) with ((n - k) * (n - k - 1)!) by nia; equality.
+  Qed.
+
   Lemma bcoeff_correct: forall n k, k <= n -> bcoeff n k = C n k.
   Proof.
     induct k; simplify.
-  Admitted.
+    symmetry; apply Cn0.
+    rewrite Cnk_1.
+    unfold_recurse (bcoeff n) k.
+    rewrite IHk.
+    equality. linear_arithmetic.
+    linear_arithmetic.
+  Qed.
 
 
   (* All binomial coefficients for a given n *)
@@ -575,13 +703,111 @@ Module Impl.
   (* Exercise: Let's prove that all_coeffs_fast is correct.
      Note that you can assume Pascal's rule to prove this. *)
   (* HINT 1 (see Pset2Sig.v) *)
+
+  Lemma len_all_coeffs_fast: forall n, len (all_coeffs_fast n) = n + 1.
+  Proof.
+    induct n.
+    simplify. linear_arithmetic.
+
+    unfold_recurse all_coeffs_fast n.
+    simplify.
+    rewrite IHn.
+    rewrite seq_len.
+    linear_arithmetic.
+  Qed.
+
+  Lemma padded_1: forall f count i start, i < count -> ith (i+1) (1::seq f count start) = f (start + i).
+  Proof.
+    induct count; simplify.
+    - linear_arithmetic.
+
+    - unfold_recurse (seq f) count.
+      simplify.
+
+      cases i.
+      + simplify.
+        rewrite N.add_0_r.
+        reflexivity.
+
+      + replace (i + 1) with (i + 1) by reflexivity.
+        unfold_recurse ith (i+1).
+        simplify.
+        unfold_recurse ith i.
+        simplify.
+
+        assert (i < count) by linear_arithmetic.
+
+        rewrite seq_spec by assumption.
+
+        replace (start + 1 + i) with (start + (i + 1)) by linear_arithmetic.
+        reflexivity.
+  Qed.
+
+
   Lemma all_coeffs_fast_correct:
     Pascal's_rule ->
     forall n k,
       k <= n ->
       ith k (all_coeffs_fast n) = C n k.
   Proof.
-  Admitted.
+    induct n; simplify.
+
+    - replace k with 0 by linear_arithmetic.
+    equality.
+
+    - unfold_recurse all_coeffs_fast n.
+    (* unfold nextLine. *)
+
+    assert (k = 0 \/  k = n + 1 \/ 1 <= k <= n ) as Hk by linear_arithmetic;
+        cases Hk; subst.
+
+      + rewrite Cn0.
+        equality.
+      +
+        unfold nextLine.
+        rewrite padded_1.
+        replace (1+n-1) with n by linear_arithmetic.
+        rewrite IHn.
+        rewrite ith_out_of_bounds_0.
+        rewrite N.add_0_r.
+        unfold C.
+        replace (n-n) with 0 by linear_arithmetic.
+        simplify. rewrite N.mul_1_l.
+        Search(_-(_+_)).
+        rewrite N.sub_add_distr.
+        replace (n + 1 - n - 1) with 0 by linear_arithmetic.
+        simplify. rewrite N.mul_1_l.
+        Search(_/_).
+        rewrite N.div_same by (apply fact_nonzero). symmetry.
+        rewrite N.div_same by (apply fact_nonzero). equality.
+
+        rewrite len_all_coeffs_fast; linear_arithmetic.
+        linear_arithmetic.
+        rewrite len_all_coeffs_fast; linear_arithmetic.
+
+
+      + rewrite H.
+        assert (k <= n) as Hle by linear_arithmetic.
+        pose proof (IHn k Hle) as Hdk.
+
+        assert (k - 1 <= n) as Hle1 by linear_arithmetic.
+        pose proof (IHn (k - 1) Hle1) as Hdk1.
+
+        cases k.
+        ++ linear_arithmetic.
+        ++ replace (k+1-1) with k by linear_arithmetic.
+          unfold nextLine.
+          rewrite padded_1.
+          replace (1+k-1) with k by linear_arithmetic.
+          replace (1+k) with (k+1) by linear_arithmetic.
+          rewrite Hdk.
+          replace (k+1-1) with (k) in Hdk1.
+          rewrite Hdk1.
+          equality.
+          linear_arithmetic.
+          rewrite len_all_coeffs_fast. linear_arithmetic.
+        ++ linear_arithmetic.
+  Qed.
 
   (* ----- THIS IS THE END OF PSET2 ----- All exercises below this line are optional. *)
 
